CrashSafeMap

disk-betree/CrashSafe.dfy
@@ -1,7 +1,7 @@
 include "DiskBetreeInv.dfy"
 include "MapSpec.dfy"
 
-abstract module CrashableDiskBetree {
+abstract module CrashSafeDiskBetree {
   import DB : DiskBetreeInv
 
   type Constants = DB.DB.Constants
@@ -61,7 +61,73 @@ abstract module CrashableDiskBetree {
   {
     var step :| NextStep(k, s, s', step);
     if (step.EphemeralMoveStep?) {
-      DB.NextPreservesInvariant(k, s.ephemeral, s'.ephemeral);
+      DB.NextPreservesInv(k, s.ephemeral, s'.ephemeral);
+    }
+  }
+}
+
+abstract module CrashSafeMap {
+  import MS : MapSpec
+
+  type Constants = MS.Constants
+  datatype Variables<T> = Variables(persistent: MS.Variables<T>, ephemeral: MS.Variables<T>)
+
+  predicate Init(k: Constants, s: Variables)
+  {
+    && MS.Init(k, s.persistent)
+    && s.ephemeral == s.persistent
+  }
+
+  datatype Step<T> =
+    | EphemeralMoveStep
+    | SyncStep
+    | CrashStep
+
+  predicate EphemeralMove(k: Constants, s: Variables, s': Variables)
+  {
+    && s.persistent == s'.persistent
+    && MS.Inv(k, s.ephemeral)
+    && MS.Next(k, s.ephemeral, s'.ephemeral)
+  }
+
+  predicate Sync(k: Constants, s: Variables, s': Variables)
+  {
+    && s'.persistent == s.ephemeral
+    && s'.ephemeral  == s.ephemeral
+  }
+
+  predicate Crash(k: Constants, s: Variables, s': Variables)
+  {
+    && s'.persistent == s.persistent
+    && s'.ephemeral  == s.persistent
+  }
+
+  predicate NextStep(k: Constants, s: Variables, s': Variables, step: Step)
+  {
+    match step {
+      case EphemeralMoveStep => EphemeralMove(k, s, s')
+      case SyncStep => Sync(k, s, s')
+      case CrashStep => Crash(k, s, s')
+    }
+  }
+
+  predicate Next<T(!new)>(k: Constants, s: Variables, s': Variables) {
+    && exists step :: NextStep(k, s, s', step)
+  }
+
+  predicate Inv(k: Constants, s: Variables) {
+    && MS.Inv(k, s.persistent)
+    && MS.Inv(k, s.ephemeral)
+  }
+
+  lemma NextPreservesInv(k: Constants, s: Variables, s': Variables)
+  requires Inv(k, s)
+  requires Next(k, s, s')
+  ensures Inv(k, s')
+  {
+    var step :| NextStep(k, s, s', step);
+    if (step.EphemeralMoveStep?) {
+      MS.NextPreservesInv(k, s.ephemeral, s'.ephemeral);
     }
   }
 }
